define progress, add lemmas, prove decomposition

LocalLang/TypingGuarantees.lean
@@ -6,6 +6,16 @@ import LocalLang.Typing
 def EnvRespectsCtx (Γ : TypeContext) (V : Env) : Prop :=
   ∀ (x : String) (n : ℕ), V[x]? = some n → Γ[x]? = LLType.nat
 
+def CtxRespectsEnv (V : Env) (Γ : TypeContext) : Prop :=
+  ∀ x : String, Γ[x]? = some LLType.nat → x ∈ V
+
+inductive IsFuncType : LLType → Prop where
+  | func {param_tys ret_ty} : IsFuncType (.func param_tys ret_ty)
+
+def CtxRespectsDefs (defs : Definitions) (Γ : TypeContext) : Prop :=
+  ∀ f : String, (f_in_Γ : f ∈ Γ) → IsFuncType Γ[f] →
+  f ∈ defs
+
 -- TODO: prove
 -- TODO: V and Γ should be related
 theorem preservation (Γ : TypeContext) (e e' : Expr) (ty : LLType) (defs : Definitions)
@@ -35,6 +45,108 @@ theorem preservation (Γ : TypeContext) (e e' : Expr) (ty : LLType) (defs : Defi
 
 -- Progress: if TypeJdg Γ e ty, then e can take a step.
 -- TODO: formalize
+
+def Expr.simple_rec.{l} {motive : Expr → Sort l}
+     (const_case : ∀ n, motive (.const n))
+     (var_case : ∀ x, motive (.var x))
+     (bin_op_case : ∀ op lhs rhs, motive lhs → motive rhs → motive (.binOp op lhs rhs))
+     (let_in_case : ∀ name e₁ e₂, motive e₁ → motive e₂ → motive (.letIn name e₁ e₂))
+     (fun_case : ∀ f es, (∀ e', e' ∈ es → motive e') → motive (.funCall f es))
+    : (e : Expr) → motive e := go
+where go
+  | .const n => const_case n
+  | .var x => var_case x
+  | .binOp op lhs rhs => bin_op_case op lhs rhs (go lhs) (go rhs)
+  | .letIn name e₁ e₂ => let_in_case name e₁ e₂ (go e₁) (go e₂)
+  | .funCall f es => fun_case f es (fun e' _ => go e')
+
+inductive IsConst : Expr → Prop where
+  | const : IsConst (.const n)
+
+inductive IsRedex : Expr → Prop where
+  | var : IsRedex (.var x)
+  | binOp {op} : IsRedex (.binOp op (.const n₁) (.const n₂))
+  | letInConst : IsRedex (.letIn x (.const n₁) (.const n₂))
+  | funCall {es} : IsRedex (.funCall f es)
+
+inductive HasDecomposition : Expr → Prop where
+  | decomposition (e' : Expr) (ctx : Ctx) : e = ctx.fill e' → IsRedex e' → HasDecomposition e
+
+lemma is_const_or_has_decomposition : ∀ e : Expr, IsConst e ∨ HasDecomposition e := by
+  intro e
+  apply e.simple_rec
+  · intro n
+    apply Or.intro_left
+    constructor
+  · intro x
+    apply Or.intro_right
+    apply HasDecomposition.decomposition (.var x) .hole (by simp)
+    constructor
+  · intro op lhs rhs ih_lhs ih_rhs
+    apply Or.intro_right
+    cases ih_lhs with
+    | inl lhs_const =>
+      cases lhs_const
+      rename_i n₁
+      cases ih_rhs with
+      | inl rhs_const =>
+        cases rhs_const
+        rename_i n₂
+        apply HasDecomposition.decomposition (.binOp op (Expr.const n₁) (Expr.const n₂))
+          .hole (by simp)
+        constructor
+      | inr rhs_dec =>
+        let ⟨e', ctx, e_eq, e'_redex⟩ := rhs_dec
+        apply HasDecomposition.decomposition e' (.binOpRhs n₁ op ctx) (by simp [e_eq])
+        assumption
+    | inr lhs_dec =>
+      let ⟨e', ctx, e_eq, e'_redex⟩ := lhs_dec
+      apply HasDecomposition.decomposition e' (.binOpLhs ctx op rhs) (by simp [e_eq])
+      assumption
+  · intro name e₁ e₂ ih_e₁ ih_e₂
+    apply Or.intro_right
+    cases ih_e₁ with
+    | inl e₁_const =>
+      cases e₁_const
+      rename_i n₁
+      cases ih_e₂ with
+      | inl e₂_const =>
+        cases e₂_const
+        rename_i n₂
+        apply HasDecomposition.decomposition (Expr.letIn name (Expr.const n₁) (Expr.const n₂))
+          .hole (by simp)
+        constructor
+      | inr e₂_dec =>
+        let ⟨e', ctx, e_eq, e'_redex⟩ := e₂_dec
+        apply HasDecomposition.decomposition e' (.letInBody name n₁ ctx) (by simp [e_eq])
+        assumption
+    | inr e₁_dec =>
+      let ⟨e', ctx, e_eq, e'_redex⟩ := e₁_dec
+      apply HasDecomposition.decomposition e' (.letInExpr name ctx e₂) (by simp [e_eq])
+      assumption
+  · intro f es ih_es
+    apply Or.intro_right
+    apply HasDecomposition.decomposition (Expr.funCall f es) .hole (by simp)
+    constructor
+
+lemma redex_progress : ∀ {defs Γ e ty}, TypeJdg Γ e ty → IsRedex e →
+  CtxRespectsEnv V Γ →  CtxRespectsDefs defs Γ →
+  ∃ e', HeadSmallStep defs V e e' := by
+  intro defs Γ e ty e_jdg e_redex V_resp_Γ defs_resp_Γ
+  -- cases e_redex with
+  -- | var =>
+  --   cases e_jdg
+  --   rename_i x x_ty
+  --   sorry
+  --   -- let _ := V_resp_Γ x x_ty
+  sorry
+
+theorem progress {Γ : TypeContext} {ty : LLType} {defs : Definitions}
+  : TypeJdg Γ e ty → CtxRespectsEnv V Γ → CtxRespectsDefs defs Γ →
+    IsConst e ∨ ∃ e', SmallStep defs V e e' := by
+  intro e_jdg V_ext_Γ
+
+  sorry
 
 -- TODO: Also interesting:
 -- if TypeJdg Γ e ty, then eval e succeeds
